

Student No :

Date :

Name & Surname :

Signature :

Q1) Find the Laplace and the inverse Laplace transform of the following functions.

(a) $\mathcal{L}\left\{e^{-7t} + 3\sin(2t) - 5\cos(4t)\right\}$

(b) $\mathcal{L}\left\{t^2e^{3t} - \sin(3t)e^{2t} + 4\cos(t)e^{-6t}\right\}$

(c) $\mathcal{L}^{-1}\left\{\frac{6}{s^4} + \frac{7}{s^2 + 49} + \frac{5}{s + 3}\right\}$

(d) $\mathcal{L}^{-1}\left\{\frac{7s^3 + 18s - 15}{(s^2 - 1)(s^2 + 4)}\right\}$

(e) $\mathcal{L}^{-1}\left\{\frac{2s}{s^2 + 8s + 17}\right\}$

(f) $\mathcal{L}^{-1}\left\{\frac{7s e^{3s}}{s^2 + 4}\right\}$

(g) $\mathcal{L}^{-1}\left\{e^{-3s}\frac{1}{s^2 + 4} + e^{4s}\frac{s}{s^2 + 1}\right\}$

Q2) Use Laplace transform to solve the initial value problem

$$-2y' + y = 0; \quad y(0) = 1$$

Q3) Use Laplace transform to solve the initial value problem

$$y'' - 4y' + 4y = 8t; \quad y(0) = 5, y'(0) = 0$$

Q4) Use Laplace transform to solve the initial value problem

$$y'' + y' = 6e^{2t}; \quad y(0) = 0, y'(0) = 3$$

Q5) Use the Laplace transform to solve the initial value problem

$$y'' + y = \cos 2t; \quad y(0) = 0, y'(0) = 1$$

Q6) Use the Laplace transform to solve the initial value problem

$$y'' - 6y' + 9y = 50\cos t; \quad y(0) = 2, y'(0) = 0$$

Q7) Use the Laplace transform to solve the initial value problem

$$y'' - 2y' + y = te^{2t}; \quad y(0) = 2, y'(0) = 6$$

Q8) Find $\mathcal{L}\left\{(t^2 - t + 5)H(t - 3)\right\}$

Q9) Find Laplace transform of the following function:

$$f(t) = \begin{cases} 0 & \text{if } t < 2 \\ t^2 - t & \text{if } t \geq 2 \end{cases}$$

Q10) Use Laplace transform to solve the initial value problem:

$$y'' + 4y = f(t), \quad y(0) = 0, y'(0) = 0, \text{ where}$$

$$f(t) = \begin{cases} 0 & \text{if } t < 3 \\ 8t - 20 & \text{if } t \geq 3 \end{cases}$$

$\mathbf{f(t)}$	$\mathcal{L}[f](s)$
e^{at}	$\frac{1}{s-a}$
t^n	$\frac{n!}{s^{n+1}}$
$\sin bt$	$\frac{b}{s^2 + b^2}$
$\cos bt$	$\frac{s}{s^2 + b^2}$

$$\mathcal{L}[y'] = sY(s) - y(0)$$

$$\mathcal{L}[y''] = s^2Y(s) - sy(0) - y'(0)$$

Shifting Theorems:

$$\mathcal{L}[e^{ct}f(t)](s) = F(s-c)$$

$$\mathcal{L}[H(t-a)f(t-a)](s) = e^{-as}\mathcal{L}[f(t)](s) = e^{-as}F(s)$$

$$H(t-a)f(t-a) = \mathcal{L}^{-1}[e^{-as}F(s)]$$